\documentclass[NumTh.tex]{subfiles}
\begin{document}

\subsection{Estimates for $\zeta(s)$:}
\begin{theorem}
  If $s = \sigma + it$.
  \begin{enumerate}
    \item Let $m \in \N_0$. Then there exists a $C_m > 0$ such that $\abs{\zeta^{(m)}(s)} \leq C_m \abs{t}$ for $\sigma > 1$ and $\abs{t} \geq 1$.
    \item There exists $c_0 > 0$ such that $\abs{ \zeta(s)} \geq c_0 \abs{t}^{-4}$ for $\sigma > 1$ and $\abs{t} \geq 1$.
  \end{enumerate}
\end{theorem}

\begin{proof}
  \begin{enumerate}
    \item $\sigma \geq 2$: 
    \begin{align*}
      \zeta^{(m)}(s) &= \sum_{n=1}^\infty ( \frac{\partial}{\partial s})^m \frac{1}{n^s} \\
      &= \sum_{n=1}^\infty \frac{(-1)^m (\log n)^m}{n^s}
    \end{align*}
    so $\abs{\zeta^{(m)}(s)} \leq \sum_{n=1}^\infty \frac{(\log n)^m}{n^2} < \infty$.
    choose $C_m$ large enough.\\
    $1 < \sigma < 2$: we already know
    \begin{align*}
      \zeta(s) = \frac{1}{s-1} + \sum_{n=1}^\infty \int_n^{n+1} ( \frac{1}{n^s} - \frac{1}{x^s}) dx \\
      \text{The sum converges uniformly in $s$.} \\
      \implies \zeta^{(m)}(s) = \frac{(-1)^m m!}{(s-1)^{m+1}} + \sum_{n=1}^\infty (-1)^m \int_n^{n+1} (\frac{(\log n)^m}{n^s} - \frac{(\log x)^m}{x^s}) dx
    \end{align*}
    Now consider
    \todo{check inequality; especially $x$ and $n$, which is right??}
    \begin{align*}
      \abs{ \frac{(\log n)^m}{n^s} - \frac{(\log x)^m}{x^s} } = \abs{ \int_{u=n}^x ( \frac{(\log u)^m}{u^s})^\prime du} 
      \leq 1 \cdot (\abs{s} + m) \frac{(\log n)^m}{x^{\sigma +1}} \leq (\abs{s}+m) \frac{(\log n)^m}{x^2} \\
    \end{align*}
    Since
    \begin{align*}
      {(\frac{(\log x)^m}{x^s})^\prime = \frac{m (\log x)^{m-1}}{x^{s+1}} - s \frac{(\log x)^m}{x^{s+1}} 
      = \frac{1}{x^{s+1}} (m (\log x)^{m-1} - s(\log x)^m)}
    \end{align*}
    \begin{align*}
      \implies \abs{\zeta^{(m)}(s)} \leq \underbrace{\frac{m!}{\abs{s-1}^{m+1}}}_{\leq m! \text{, } \abs{s-1} \geq \abs{t} \geq 1} + C_m^\prime \abs{s} \underbrace{\sum_{n=1}^\infty \frac{(\log n)^m}{n^2}}_{< \infty} \leq C_m^{\prime \prime} \abs{s} \leq C_m \abs{t}
    \end{align*}
    since $\abs{s} \leq \underbrace{\sigma}_{\in (1,2)} + \underbrace{\abs{t}}_{\geq 1}$
    \item Let $\sigma > 1$.
    \begin{align*}
      \log \zeta(s) = \sum_p - \log (1-p^{-s}) \overset{- \log (1-z) = \sum_{n=1}^\infty \frac{z^n}{n} \text{ for } \abs{z} < 1}{=}
      \sum_p \sum_\nu \frac{1}{\nu p^{\nu s}}
      = \sum_n \frac{b_n}{n^s}
    \end{align*}
    where $ b_n \coloneq \begin{cases}
      \frac{1}{\nu}, & \text{if } n = p^\nu, p \text{ prime} \\
      0, & \text{otherwise}
    \end{cases} $
  \end{enumerate}
  Let 
  \[ B(s) \coloneq \sum_{n=1}^\infty \frac{b_n}{n^s} \]
  In other words,
  \[ \zeta(s) = e^{B(s)} \]
  for $\sigma > 1$.
  \begin{lemma}\label{lt2}
    Let $B(s) = \sum_{n=1}^\infty \frac{b_n}{n^s}$ be a D-series with $b_n \geq 0$, that is (abs) convergent for $\sigma > 1$.
    Then $Re(B(\sigma + 2 it)) + 4 \cdot Re(B(\sigma+it)) + 3 \cdot Re(B(\sigma)) \geq 0$ for $\sigma > 1$.
    In particular, for $Z(s) \coloneq e^{B(s)}$, we have
    \[ \abs{Z(\sigma +it)}^4 \cdot \abs{Z(\sigma +2 it)} \cdot \abs{Z(\sigma)}^3 \geq 1 \]
  \end{lemma}
  \begin{proof}
    Let $a \in \C$, $a \overbar{a} = \abs{a} =1$.
    Then 
    \begin{align*}
      (a + \overbar{a})^4 &= \sum_{j=0}^4 \left( 4 \choose j \right) a^j \overbar{a}^{4-j} \\
      &= \overbar{a}^4 + 4 \overbar{a}^2 + 6  + 4 a^2 + a^4 \\
      &= (a^4 + \overbar{a}^4) + 4( a^2 + \overbar{a}^2) + 6
    \end{align*}
    $a + \overbar{a} = 2 Re(a)$
    \begin{align*}
      0 \leq 16 Re(a)^4 = 2 Re(a^4) + 8 Re(a^2) +6 \\
      \implies Re(a^4) + 4 Re(a^2) +3  = 8 Re(a)^4 \geq 0
    \end{align*}
    Choose $a \coloneq n^{- \frac{it}{2}}$. Then we get
    \begin{align*}
      Re(n^{-2it}) + 4 Re(n^{-it}) + 3 \geq 0
    \end{align*}
    Multiply this by $\frac{b_n}{n^\sigma}$
    \begin{align*}
      Re(\frac{b_n}{n^{\sigma + 2it}} + 4 Re(\frac{b_n}{n^{\sigma + it}} + 3 Re(\frac{b_n}{n^\sigma}) \geq 0 \text{ take the sum over all n}\\
      Re(B(\sigma + 2it)) + 4 Re(B(\sigma + it)) + 3 Re(B(\sigma)) \geq 0 \text{ use } e^\bullet \\
      \abs{Z(\sigma + 2it)} \cdot \abs{Z(\sigma + it)}^4 \cdot \abs{Z(\sigma)}^3 \geq 1
    \end{align*}
  \end{proof}
  Applying this to $Z(s) = \zeta(s) = e^{B(s)}$, we get
  \begin{align} \label{star}
    \abs{\frac{\zeta(\sigma + it)}{\sigma - 1}}^4 \cdot \abs{\zeta(\sigma + 2it)} \cdot \abs{\zeta(\sigma)(\sigma-1)}^3 \geq \frac{1}{\sigma - 1}
  \end{align}
  \begin{rem}
    \ref{star} implies $\zeta(s) \neq 0$ or $\sigma = 1$.
    Indeed, assume $\zeta(1+it) = 0, t\neq 0$. Then
    \begin{align*}
      \lim_{\sigma \searrow 1} LHS &=  \lim_{\sigma \searrow 1} \abs{\frac{\zeta(\sigma+it) - \zeta(1+it)}{\sigma - 1}}^4 \cdot \lim_{\sigma \searrow 1} \abs{\zeta(\sigma + 2it)} \lim_{\sigma \searrow 1} \abs{\zeta(\sigma)(\sigma -1)}^3 \\
      &= \abs{\zeta^\prime(1+it)^4 \zeta(1+2it) \cdot 1} < \infty
    \end{align*}
    But $\lim_{\sigma \searrow 1} RHS = \infty$ and thus $\lightning$.
  \end{rem}
  Assume first that $\sigma \geq 2$.
  Then 
  \begin{align*}
    \abs{\zeta(s)} \geq 1 - \abs{\zeta(s) - 1} = 1 - \abs{\sum_{n=2}^\infty \frac{1}{n^s}}
    \geq 1 - \sum_{n=2}^\infty \frac{1}{n^2}
    = 1 - (\zeta(2) - 1) = 2 -\zeta(2) > 0
  \end{align*}
  \begin{lemma}
    $\zeta(2) = \frac{\pi^2}{6} \approx 1,64 < 2$
  \end{lemma}
  \begin{proof}[Proof by Euler]
    WeierstaÃŸ product for $\sin(\pi x)$.
    \begin{align*}
      \sin(\pi x) = \pi x \prod_{n=1}^\infty (1 - \frac{x^2}{n^2})
    \end{align*}
    \begin{align*}
      \sin(\pi x) = \pi x - \frac{(\pi x)^3}{3!} + \dots \\
      \implies \pi  x \prod_{n=1}^\infty (1- \frac{x^2}{n^2}) = \pi x - (\pi x)^3 \sum_{n=1}^\infty \frac{1}{n^2} + \dots
    \end{align*}
    comparison with the coefficient of $[x^3]$ yields
    \begin{align*}
      \frac{(\pi x)^3}{6} = \pi x^3 \zeta(2) \\
      \implies \zeta(2) = \frac{\pi^2}{6}
    \end{align*}
  \end{proof}
  $1 < \sigma < 2$: Rewrite \ref{star} with $s = \sigma +it$.
  \begin{align*}
    \abs{\zeta(s)} \geq (\sigma - 1)^{\frac{3}{4}} \abs{\zeta(\sigma + 2it)}^{-\frac{1}{4}} \cdot \abs{\zeta(\sigma) (\sigma-1)}^{-\frac{3}{4}}
  \end{align*}
  The function $\sigma \mapsto (\sigma - 1) \zeta(\sigma)$ is continuous on $1 \leq \sigma \leq 2$, we see in $1 \leq \sigma \leq 2$ that $c_2 \geq \abs{\zeta(\sigma) (\sigma -1) } \geq c_1 > 0$ for some $c_1$ (compactness)\\
  By 1) $\implies \abs{\zeta(\sigma + 2it)} \leq 2 C_0 \abs{t}$, $\abs{t} \geq 1$.
  Therefore:
  \begin{align} \label{starstar}
    \abs{\zeta(s)} \geq A(\sigma - 1)^{\frac{3}{4}} \abs{t}^{-\frac{1}{4}} 
  \end{align}
  where $A > 0$, for $1 < \sigma < 2$ and $\abs{t} \geq 1$.
  Let $\varepsilon \in (0,1)$ small enough (see later)
  Define
  \[ \sigma(t) \coloneq 1 + \varepsilon \abs{t}^{-5} \in (1,2) \text{ for } \abs{t} \geq 1 \]
  Case a) $\sigma \geq \sigma(t)$.
  Then \ref{starstar} implies that 
  \[ \abs{\zeta(s)} \geq A (\varepsilon \abs{t}^{-5})^{\frac{3}{4}} \abs{t}^{-\frac{1}{4}} = A \varepsilon^{\frac{3}{4}} \abs{t}^{-4} \checkmark \]
  Case b) $1 < \sigma < \sigma(t)$.
  Then 
  \begin{align*}
    \zeta(s) = \zeta(\sigma + it) = \zeta(\sigma(t) + it) - \int_\sigma^{\sigma(t)} \zeta^\prime(x + it) dx \\
    \implies \abs{\zeta(s)} \geq \abs{\zeta(\sigma(t) + it)} - \abs{\int_\sigma^{\sigma(t)} \zeta^\prime(x + it) dx} \\
    1) \implies \abs{\zeta^\prime(x + it)} \leq C_1 \abs{t} \\
    \implies \abs{\zeta(s)} \geq \abs{\zeta(\sigma(t) + it)} - C_1 \abs{t} (\sigma(t) -1) 
    \overset{\ref{starstar}}{\geq} A (\sigma(t) - 1)^{\frac{3}{4}} \abs{t}^{-\frac{1}{4}} - C_1 \abs{t} (\sigma(t) -1) \\
    \geq A \varepsilon^{\frac{3}{4}} \abs{t}^{-4} - C_1 \varepsilon \abs{t}^{-4}
    = \underbrace{(A \varepsilon^{\frac{3}{4}}}_{\text{choose $\varepsilon$ small enough to ensure that this is $>0$}} - C_1 \varepsilon) \abs{t}^{-4}
  \end{align*}
\end{proof}


\end{document}
